Quantify Enums over Set, get rid of type/tdenote
in exchange we depend on an axiom: UIP aka the K axiom.

The alternative would be to only quantify Enum over Sets with decidable
equality, but the mechanics of doing this would clutter the development
for what is ultimately not that important.

On the other hand it might be possible to go without UIP/K/JMeq entirely
using similar techniques described at the end of
http://adam.chlipala.net/cpdt/html/Universes.html but my Coq Fu is too
weak.

model/Enum.v
@@ -2,7 +2,7 @@ Require Import Coq.Arith.Arith_base  Coq.Arith.Div2.
 Require Import Coq.Lists.ListSet Coq.Lists.List.
 Require Import Coq.Numbers.Natural.Peano.NPeano.
 
-Require Import Bijection Pairing Sets Trace Typ Util.
+Require Import Bijection Pairing Sets Trace Util.
 
 (* Notation notes:
 Sets
@@ -19,17 +19,17 @@ Traces
 ≡ \equiv    trace_eq
  *)
 
-Inductive Enum : type -> Set :=
-| E_Nat : Enum TNat
-| E_Pair {tl tr} : Enum tl -> Enum tr -> Enum (TPair tl tr)
-| E_Map {tyin tyout} : Bijection (tdenote tyout) (tdenote tyin) -> Enum tyin -> Enum tyout
-| E_Dep {t1 t2} : Enum t1 -> (tdenote t1 -> Enum t2) -> Enum (TPair t1 t2)
-| E_Sum {tl tr} : Enum tl -> Enum tr -> Enum (TSum tl tr)
+Inductive Enum : Set -> Type :=
+| E_Nat : Enum nat
+| E_Pair {tl tr} : Enum tl -> Enum tr -> Enum (tl * tr)
+| E_Map {tyin tyout} : Bijection tyout tyin -> Enum tyin -> Enum tyout
+| E_Dep {t1 t2} : Enum t1 -> (t1 -> Enum t2) -> Enum (t1 * t2)
+| E_Sum {tl tr} : Enum tl -> Enum tr -> Enum (tl + tr)
 | E_Trace {t} : tag -> Enum t -> Enum t (* A no-op wrapper to signal tracing *)
 .
 Hint Constructors Enum.
 
-Inductive Enumerates : forall {t : type}, Enum t -> nat -> tdenote t -> Trace -> Prop :=
+Inductive Enumerates : forall {T : Set}, Enum T -> nat -> T -> Trace -> Prop :=
 | ES_Nat :
     forall n,
       Enumerates E_Nat n n ε
@@ -40,12 +40,12 @@ Inductive Enumerates : forall {t : type}, Enum t -> nat -> tdenote t -> Trace ->
       Enumerates r rn rx rt ->
       Enumerates (E_Pair l r) n (lx, rx) (lt ⊔ rt)
 | ES_Map :
-    forall {tl tr} (bi : Bijection (tdenote tl) (tdenote tr)) inner inner_x n x t,
+    forall {tl tr} (bi : Bijection tl tr) inner inner_x n x t,
       Bijects bi x inner_x ->
       Enumerates inner n inner_x t ->
       Enumerates (E_Map bi inner) n x t
 | ES_Dep:
-    forall {tl tr} (l: Enum tl) (f: tdenote tl -> Enum tr) n ln rn lx rx lt rt,
+    forall {tl tr} (l: Enum tl) (f: tl -> Enum tr) n ln rn lx rx lt rt,
       Pairing n ln rn ->
       Enumerates l ln lx lt ->
       Enumerates (f lx) rn rx rt ->
@@ -115,7 +115,7 @@ Ltac invert_Enumerates' :=
       end
   end.
 
-Ltac invert_Enumerates := repeat invert_Enumerates'; repeat dec_K.
+Ltac invert_Enumerates := repeat invert_Enumerates'; repeat destruct_eq.
 
 Ltac odd_neq_event :=
   match goal with
@@ -150,7 +150,7 @@ Proof.
           |- _ ] => destruct (IH _ _ _ _ _ _ H1 H2); clear IH H1 H2; subst
       end;
   repeat Eff_indHyp;
-  tauto.
+  try tauto.
 Qed.
 
 Ltac Etf_indHyp :=
@@ -170,7 +170,7 @@ Theorem Enumerates_to_fun :
 Proof.
   induction e; intros;
   repeat invert_Enumerates; try sumbool_contra;
-  repeat destruct_eq; repeat Etf_indHyp; repeat rewrite_pairing_from_fun; try rewrite_biject_funr;
+  repeat Etf_indHyp; repeat rewrite_pairing_from_fun; try rewrite_biject_funr;
   try match goal with
         | [ IH: context[Enumerates _ _ _ _ -> Enumerates _ _ _ _ -> _ ]
           , H1 : Enumerates ?e _ _ _
@@ -212,7 +212,7 @@ Ltac Etd_indHyp :=
 
 (* Map/Trace compatibility lemmas *)
 Lemma Enumerates_to_dec_Map :
-  forall tyin tyout (b: Bijection (tdenote tyin) (tdenote tyout)) e x,
+  forall tyin tyout (b: Bijection tyin tyout) e x,
     (forall x, { nt: nat * Trace | let (n, t) := nt in Enumerates e n x t }) ->
     { nt : nat * Trace | let (n, t) := nt in Enumerates (E_Map b e) n x t }.
 Proof.
@@ -230,7 +230,7 @@ Definition Enumerates_to_dec:
 Proof.
   induction e; intros; auto;
   try (eexists (_, _); eauto; fail);
-  tdenote_crush; repeat Etd_indHyp; (eexists (_, _); eauto).
+  inj_crush; repeat Etd_indHyp; (eexists (_, _); eauto).
 Defined.
 
 Definition Enumerates_to_dec_uniq :
@@ -275,10 +275,10 @@ Proof.
 Defined.
 
 Definition Enumerates_from_dec:
-  forall {ty} (e: Enum ty) n,
-    { xt : tdenote ty * Trace | let (x, t) := xt in Enumerates e n x t }.
+  forall {ty: Set} (e: Enum ty) n,
+    { xt : ty * Trace | let (x, t) := xt in Enumerates e n x t }.
 Proof.
-  refine (fix F {ty} e n : { xt : tdenote ty * Trace | let (x, t) := xt in Enumerates e n x t } :=
+  refine (fix F {ty : Set} e n : { xt : ty * Trace | let (x, t) := xt in Enumerates e n x t } :=
             match e with
               | E_Nat  => {{(n, ε)}}
               | E_Pair _ _ el er =>
@@ -324,12 +324,12 @@ Proof.
                   | {{ xt }} =>
                     {{ (fst xt, trace_one n tg)}}
                 end
-            end); clear F; tdenote_crush; eauto.
+            end); clear F; inj_crush; eauto.
 Defined.
 
 Definition Enumerates_from_dec_uniq :
   forall {ty} (e: Enum ty) n,
-  exists ! (xt : tdenote ty * Trace),
+  exists ! (xt : ty * Trace),
     let (x, t) := xt
     in Enumerates e n x t.
 Proof.
@@ -554,7 +554,7 @@ Theorem trace_lt_Nat n tg
 : z_to_n n ≃ trace_proj tg (Trace_lt (E_Trace tg E_Nat) n).
 Proof.
   induction n as [| n IHn]; [destruct tg; compute; tauto|].
-  unfold Trace_lt. fold (@Trace_lt TNat).
+  unfold Trace_lt. fold (@Trace_lt nat).
   unfold z_to_n. fold z_to_n.
   rewrite trace_proj_plus_distrl.
   rewrite Trace_nat.
@@ -574,7 +574,7 @@ Proof.
   intros Hdiff.
   induction n.
   destruct tg1; auto.
-  unfold Trace_lt; fold (@Trace_lt TNat).
+  unfold Trace_lt; fold (@Trace_lt nat).
   rewrite trace_proj_plus_distrl.
   rewrite trace_off.
   rewrite IHn; compute; auto.
@@ -658,7 +658,7 @@ Theorem trace_lt_Pair_off {tyl tyr} tg (e1 : Enum tyl) (e2 : Enum tyr) m
 Proof.
   induction m; [intros; destruct tg; reflexivity|].
   intros H1 H2.
-  unfold Trace_lt; fold (@Trace_lt (TPair tyl tyr)).
+  unfold Trace_lt; fold (@Trace_lt (tyl * tyr)).
   rewrite trace_proj_plus_distrl.
   apply subset_nil_nil.
   apply subset_union_both.
@@ -682,7 +682,7 @@ Theorem trace_lt_Sum_off {tyl tyr} tg (e1 : Enum tyl) (e2 : Enum tyr) m
   -> trace_proj tg (Trace_lt (E_Sum e1 e2) m) = ∅.
 Proof.
   induction m; [intros; compute; destruct tg; trivial|];
-  intros; unfold Trace_lt; (fold (@Trace_lt (TSum tyl tyr))); rewrite trace_proj_plus_distrl;
+  intros; unfold Trace_lt; (fold (@Trace_lt (tyl + tyr))); rewrite trace_proj_plus_distrl;
   rewrite IHm; auto; apply trace_on_Sum_off; auto.
 Qed.
 
